proof/invariant-abstract/ARM/ArchDetSchedDomainTime_AI.thy
@@ -22,7 +22,7 @@ crunch domain_list_inv [wp, DetSchedDomainTime_AI_assms]: arch_finalise_cap "\<l
 crunch domain_list_inv [wp, DetSchedDomainTime_AI_assms]:
   arch_activate_idle_thread, arch_switch_to_thread, arch_switch_to_idle_thread,
   handle_arch_fault_reply, init_arch_objects, arch_tcb_set_ipc_buffer,
-  arch_invoke_irq_control, handle_vm_fault,
+  arch_invoke_irq_control, handle_vm_fault, arch_get_sanitise_register_info,
   prepare_thread_delete, handle_hypervisor_fault
   "\<lambda>s. P (domain_list s)"
 
@@ -35,7 +35,7 @@ crunch domain_time_inv [wp, DetSchedDomainTime_AI_assms]: arch_finalise_cap "\<l
 crunch domain_time_inv [wp, DetSchedDomainTime_AI_assms]:
   arch_activate_idle_thread, arch_switch_to_thread, arch_switch_to_idle_thread,
   handle_arch_fault_reply, init_arch_objects, arch_tcb_set_ipc_buffer,
-  arch_invoke_irq_control, handle_vm_fault,
+  arch_invoke_irq_control, handle_vm_fault, arch_get_sanitise_register_info,
   prepare_thread_delete, handle_hypervisor_fault
   "\<lambda>s. P (domain_time s)"
 
