proof/invariant-abstract/Tcb_AI.thy
@@ -24,6 +24,15 @@ locale Tcb_AI_1 =
   assumes same_object_obj_refs:
   "\<And>cap cap'. \<lbrakk> same_object_as cap cap' \<rbrakk>
      \<Longrightarrow> obj_refs cap = obj_refs cap'"
+  assumes arch_get_sanitise_register_info_invs[wp]:
+  "\<And>t. \<lbrace>\<lambda>(s::'state_ext state). invs s\<rbrace> arch_get_sanitise_register_info t
+       \<lbrace>\<lambda>b s. invs s\<rbrace>"
+  assumes arch_get_sanitise_register_info_tcb_at[wp]:
+  "\<And>t a. \<lbrace>\<lambda>(s::'state_ext state). tcb_at a s\<rbrace> arch_get_sanitise_register_info t
+       \<lbrace>\<lambda>b s. tcb_at a s\<rbrace>"
+  assumes arch_get_sanitise_register_info_ex_nonz_cap_to[wp]:
+  "\<And>t a. \<lbrace>\<lambda>(s::'state_ext state). ex_nonz_cap_to a s\<rbrace> arch_get_sanitise_register_info t
+       \<lbrace>\<lambda>b s. ex_nonz_cap_to a s\<rbrace>"
   assumes finalise_cap_not_cte_wp_at:
   "\<And>P cap fin. P cap.NullCap \<Longrightarrow> \<lbrace>\<lambda>(s::'state_ext state). \<forall>cp \<in> ran (caps_of_state s). P cp\<rbrace>
                 finalise_cap cap fin \<lbrace>\<lambda>rv s. \<forall>cp \<in> ran (caps_of_state s). P cp\<rbrace>"
@@ -148,11 +157,11 @@ lemma readreg_invs:
      (clarsimp simp: invs_def valid_state_def valid_pspace_def
               dest!: idle_no_ex_cap)
 
-lemma writereg_invs:
-  "\<lbrace>invs and tcb_at dest and ex_nonz_cap_to dest\<rbrace>
+lemma (in Tcb_AI_1) writereg_invs:
+  "\<lbrace>(invs::'state_ext::state_ext state \<Rightarrow> bool) and tcb_at dest and ex_nonz_cap_to dest\<rbrace>
      invoke_tcb (tcb_invocation.WriteRegisters dest resume values arch)
    \<lbrace>\<lambda>rv. invs\<rbrace>"
-  by (wpsimp|rule conjI)+
+  by (wpsimp |rule conjI)+
 
 lemma copyreg_invs:
   "\<lbrace>invs and tcb_at src and tcb_at dest and ex_nonz_cap_to dest and
